theories/MaxOfTwoNumbersSimpler/Heuristics.v
@@ -1,0 +1,30 @@
+From Coq Require Import String Floats Uint63 NArith QArith ZArith Lia List.
+Local Open Scope float_scope.
+Local Open Scope string_scope.
+Local Open Scope list_scope.
+Local Open Scope uint63_scope.
+Import ListNotations.
+
+#[local] Set Warnings Append "-inexact-float".
+(*
+Definition incorrect_results : list (list int)
+  := [[ 3;  2];
+      [ 6;  5];
+      [ 7;  8];
+      [13; 12];
+      [15; 14];
+      [17; 16];
+      [22; 23];
+      [22; 26];
+      [24; 26];
+      [25; 26];
+      [30; 31];
+      [34; 37];
+      [36; 37];
+      [36; 38];
+      [41; 42];
+      [41; 43];
+      [42; 41];
+      [48; 49];
+      [50; 51]].
+*)
