theories/MaxOfTwoNumbersSimpler/Model.v
@@ -1,0 +1,392 @@
+From Coq Require Import Floats Sint63 Uint63 QArith Lia List PArray Morphisms RelationClasses.
+From NeuralNetInterp.Util Require Import Default Pointed PArray List Notations Arith.Classes Arith.Instances Bool.
+From NeuralNetInterp.Util Require Nat Wf_Uint63.
+From NeuralNetInterp.Torch Require Import Tensor Einsum Slicing.
+From NeuralNetInterp.TransformerLens Require Import HookedTransformer.
+From NeuralNetInterp.MaxOfTwoNumbers Require Import Parameters.
+Import Util.Nat.Notations.
+Import Util.Wf_Uint63.LoopNotation.
+Import Util.Wf_Uint63.
+Import Util.Wf_Uint63.Reduction.
+Import Arith.Instances.Truncating.
+Local Open Scope float_scope.
+Local Open Scope list_scope.
+Set Implicit Arguments.
+Import ListNotations.
+Local Open Scope raw_tensor_scope.
+
+(* Based on https://colab.research.google.com/drive/1N4iPEyBVuctveCA0Zre92SpfgH6nmHXY#scrollTo=Q1h45HnKi-43, Taking the minimum or maximum of two ints *)
+
+(** Coq infra *)
+#[local] Coercion Uint63.of_Z : Z >-> Uint63.int.
+
+(** Hyperparameters *)
+Definition N_LAYERS : nat := 1.
+Definition N_HEADS : nat := 1.
+Definition D_MODEL : nat := 32.
+Definition D_HEAD : nat := 32.
+(*Definition D_MLP = None*)
+
+Definition D_VOCAB : nat := 64.
+
+Notation tensor_of_list ls := (Tensor.PArray.abstract (Tensor.PArray.concretize (Tensor.of_list ls))) (only parsing).
+Definition W_E : tensor _ _ := Eval cbv in tensor_of_list MaxOfTwoNumbers.Parameters.W_E.
+Definition W_pos : tensor _ _ := Eval cbv in tensor_of_list MaxOfTwoNumbers.Parameters.W_pos.
+Definition L0_attn_W_Q : tensor _ _ := Eval cbv in tensor_of_list MaxOfTwoNumbers.Parameters.L0_attn_W_Q.
+Definition L0_attn_W_K : tensor _ _ := Eval cbv in tensor_of_list MaxOfTwoNumbers.Parameters.L0_attn_W_K.
+Definition L0_attn_W_V : tensor _ _ := Eval cbv in tensor_of_list MaxOfTwoNumbers.Parameters.L0_attn_W_V.
+Definition L0_attn_W_O : tensor _ _ := Eval cbv in tensor_of_list MaxOfTwoNumbers.Parameters.L0_attn_W_O.
+Definition L0_attn_b_Q : tensor _ _ := Eval cbv in tensor_of_list MaxOfTwoNumbers.Parameters.L0_attn_b_Q.
+Definition L0_attn_b_K : tensor _ _ := Eval cbv in tensor_of_list MaxOfTwoNumbers.Parameters.L0_attn_b_K.
+Definition L0_attn_b_V : tensor _ _ := Eval cbv in tensor_of_list MaxOfTwoNumbers.Parameters.L0_attn_b_V.
+Definition L0_attn_b_O : tensor _ _ := Eval cbv in tensor_of_list MaxOfTwoNumbers.Parameters.L0_attn_b_O.
+Definition L0_ln1_b : tensor _ _ := Eval cbv in tensor_of_list MaxOfTwoNumbers.Parameters.L0_ln1_b.
+Definition L0_ln1_w : tensor _ _ := Eval cbv in tensor_of_list MaxOfTwoNumbers.Parameters.L0_ln1_w.
+Definition ln_final_b : tensor _ _ := Eval cbv in tensor_of_list MaxOfTwoNumbers.Parameters.ln_final_b.
+Definition ln_final_w : tensor _ _ := Eval cbv in tensor_of_list MaxOfTwoNumbers.Parameters.ln_final_w.
+Definition W_U : tensor _ _ := Eval cbv in tensor_of_list MaxOfTwoNumbers.Parameters.W_U.
+Definition b_U : tensor _ _ := Eval cbv in tensor_of_list MaxOfTwoNumbers.Parameters.b_U.
+
+#[local] Notation FLOAT := float (only parsing). (* or Q *)
+
+Section with_batch.
+  Context {r} {batch : Shape r} {pos}
+    (s := (batch ::' pos)%shape)
+    (resid_shape := (s ::' cfg.d_model)%shape).
+
+  Definition embed (tokens : tensor IndexType s) : tensor FLOAT resid_shape
+    := HookedTransformer.embed W_E tokens.
+
+  Definition pos_embed (tokens : tensor IndexType s) : tensor FLOAT resid_shape
+    := HookedTransformer.pos_embed (n_ctx:=cfg.n_ctx) W_pos tokens.
+
+  Definition ln_final (resid : tensor FLOAT resid_shape) : tensor FLOAT resid_shape
+    := HookedTransformer.ln_final cfg.eps ln_final_w ln_final_b resid.
+
+  Definition unembed (resid : tensor FLOAT resid_shape) : tensor FLOAT (s ::' cfg.d_vocab_out)
+    := HookedTransformer.unembed W_U b_U resid.
+
+  Definition blocks_params : list _
+    := [(L0_attn_W_Q, L0_attn_W_K, L0_attn_W_V, L0_attn_W_O,
+          L0_attn_b_Q, L0_attn_b_K, L0_attn_b_V,
+          L0_attn_b_O,
+          L0_ln1_w, L0_ln1_b)].
+
+  Definition logits (tokens : tensor IndexType s) : tensor FLOAT (s ::' cfg.d_vocab_out)
+    := HookedTransformer.logits
+         (n_ctx:=cfg.n_ctx)
+         cfg.eps
+         W_E
+         W_pos
+
+         blocks_params
+
+         ln_final_w ln_final_b
+
+         W_U b_U
+
+         tokens.
+End with_batch.
+
+Notation model := logits (only parsing).
+
+Definition loss_fn {r} {batch : Shape r} {return_per_token : with_default "return_per_token" bool false}
+  (logits : tensor FLOAT (batch ::' cfg.n_ctx ::' cfg.d_vocab_out))
+  (tokens : tensor IndexType (batch ::' cfg.n_ctx))
+  : tensor FLOAT (if return_per_token return Shape (if return_per_token then _ else _) then Shape.squeeze batch else [])
+  := (let logits : tensor FLOAT (batch ::' _)
+        := PArray.checkpoint (logits.[…, -1, :]) in
+      let true_maximum : tensor IndexType (batch ::' 1)
+        := reduce_axis_m1 (keepdim:=true) Reduction.max tokens in
+      let log_probs
+        := log_softmax_dim_m1 logits in
+      let correct_log_probs
+        := PArray.checkpoint (gather_dim_m1 log_probs true_maximum) in
+      if return_per_token return (tensor FLOAT (if return_per_token return Shape (if return_per_token then _ else _) then _ else _))
+      then -Tensor.squeeze correct_log_probs
+      else -Tensor.mean correct_log_probs)%core.
+
+Definition acc_fn {r} {batch : Shape r} {return_per_token : with_default "return_per_token" bool false}
+  (logits : tensor FLOAT (batch ::' cfg.n_ctx ::' cfg.d_vocab_out))
+  (tokens : tensor IndexType (batch ::' cfg.n_ctx))
+  : tensor FLOAT (if return_per_token return Shape (if return_per_token then _ else _) then batch else [])
+  := (let pred_logits : tensor FLOAT (batch ::' _)
+        := PArray.checkpoint (logits.[…, -1, :]) in
+      let pred_tokens : tensor IndexType batch
+        := reduce_axis_m1 (keepdim:=false) Reduction.argmax pred_logits in
+      let true_maximum : tensor IndexType batch
+        := reduce_axis_m1 (keepdim:=false) Reduction.max tokens in
+      let res : tensor FLOAT _
+        := PArray.checkpoint (Tensor.of_bool (Tensor.map2 eqb pred_tokens true_maximum)) in
+      if return_per_token return (tensor FLOAT (if return_per_token return Shape (if return_per_token then _ else _) then _ else _))
+      then res
+      else Tensor.mean res)%core.
+
+Definition all_tokens : tensor RawIndexType [(cfg.d_vocab ^ cfg.n_ctx)%core : N; 2]
+  := let all_toks := Tensor.arange (start:=0) (Uint63.of_Z cfg.d_vocab) in
+     PArray.checkpoint (Tensor.cartesian_prod all_toks all_toks).
+
+Definition logits_all_tokens : tensor _ _
+  := logits all_tokens.
+
+(*
+Definition expected : tensor _ _ := Eval cbv in tensor_of_list [[11.4344;  0.5226;  3.3839;  1.9724;  4.5840;  0.6439;  3.9603;
+           3.0340;  0.5467; -5.0662;  3.6980; -2.9019; -0.3635;  1.2298;
+           4.1899; -1.8617;  1.8041;  1.8292;  3.8814;  1.5263; -0.3807;
+           1.7364;  0.7279;  3.1928;  1.7333;  3.0208;  2.5443; -0.7108;
+           0.9530; -2.2473; -0.9498; -2.4825;  0.0581;  3.0415;  0.8609;
+           1.0091;  1.2683; -0.3473;  0.8327;  1.0073; -4.2868; -0.1874;
+           1.8262;  0.7708;  3.0639;  2.7830;  3.9294; -1.5691; -4.2706;
+          -0.5728;  2.8097;  0.7026;  3.4807;  0.1257; -3.0862; -5.0693;
+          -0.7354; -2.0195; -4.0030; -0.7678; -2.5556; -4.7284; -3.5146;
+          -5.1069];
+         [ 6.0360; 11.5127;  4.9837;  4.2883; -1.8071;  3.2009;  4.2418;
+           4.7591;  0.7054; -1.4242; -1.3333; -1.6746;  0.3838;  2.4033;
+           3.9232;  3.2540;  0.3340; -3.2795;  4.9276;  1.1228;  2.5380;
+           3.1367;  0.6326;  2.8105;  3.6972;  1.0036;  2.2720;  2.9813;
+           1.5565;  0.4808;  3.2460; -3.2794; -4.5643;  3.1560;  2.5760;
+          -1.0905; -0.1279; -0.5574; -1.7911;  1.7425; -2.4315; -6.5479;
+          -3.5974; -1.0411; -0.4464;  0.3043;  3.2796;  2.8466; -0.4816;
+          -1.8650;  3.2621; -2.8751; -0.6053;  2.9918; -1.3914; -6.3286;
+           2.1076; -3.4658; -4.5172;  2.4994;  1.8171; -4.6102; -6.5373;
+           1.7269]].
+Time Definition result_arr : PArray.concrete_tensor _ _ := Eval vm_compute in PArray.concretize (logits (tensor_of_list [0; 1]%uint63)).
+Compute FloatArith.Definitions.PrimFloat.of_Q ((64*64)%Z * 0.3 / 60)%Q.
+Compute PArray.concretize (logits (tensor_of_list [0; 2]%uint63)).
+Definition result : tensor _ _ := PArray.abstract result_arr.
+Compute PArray.concretize (result - expected)%core.
+     = [| [| 11.434387031836676; 0.5225952099932295; 3.3839615308198665; 1.9723887274855556; 4.5840063309948658; 0.64385290801723039; 3.9602483380087743; 3.0339969681349053; 0.54666607504673503; -5.0662180322516335; 3.6979800582492062; -2.9019268688689768; -0.36348443193618468; 1.2297840763444583; 4.189857491356042; -1.8616910503821245; 1.804090211983326; 1.8292099701662567; 3.8813690053959768; 1.5262920988022219; -0.38072557083109465; 1.7363844416543817; 0.72784724183845517; 3.1928010802567672; 1.7333341503747564; 3.0208574099821242; 2.5442793427179553; -0.71076713961968063; 0.95301324929507791; -2.2472504997189153; -0.94977971836142461; -2.4825233318920228; 0.05807913103842096; 3.0415207967335487; 0.86088171076683107; 1.0090544553435303; 1.2682813303838136; -0.34728129319660128; 0.83264952656657487; 1.0073418196589397; -4.2868031462458358; -0.18743217937196893; 1.8262050705820332; 0.77080360675055126; 3.0638999117251253; 2.7829999418904188; 3.9294273712619519; -1.569034572864701; -4.2705754628179813; -0.57280493317185277; 2.8096841376280133; 0.70263283798417309; 3.4807142916345812; 0.12578831842769334; -3.0862327247845767; -5.0693239825969298; -0.73542478973588787; -2.019542098451649; -4.0029349556642133; -0.7678700145954146; -2.5555871045134904; -4.7283349691231136; -3.5146408535293845; -5.1069026943437343 |
+          0 : float |]; [| 6.0360160792287969; 11.512676855279571; 4.9837538534347781; 4.2883503470396374; -1.8070936444021086; 3.2009103630435618; 4.2417619133695368; 4.7591326589726597; 0.70535258541459811; -1.4242060544427955; -1.333349936148857; -1.6746240601861251; 0.38384530563141156; 2.4032875969141934; 3.9231751531146357; 3.2539967672919414; 0.33398775746797815; -3.2795048004284282; 4.9276337190120616; 1.1227905011618451; 2.5379588444008108; 3.1366626154120354; 0.6325305731516675; 2.8104326649687406; 3.697226302709212; 1.0036645575970651; 2.2720114597247907; 2.9813322143054646; 1.5564877554718004; 0.48082360054450995; 3.2459437139521889; -3.2794239451063349; -4.5643368221776033; 3.1560178954026767; 2.5759588667793594; -1.090506705640119; -0.12788111123705706; -0.55740134375287398; -1.7911646630792972; 1.7425475380881124; -2.4314792009789867; -6.5479038953987692; -3.5973805570082895; -1.041050854628057; -0.44637160751175065; 0.30425237776553304; 3.2796284224670003; 2.846615225248923; -0.4816249794681694; -1.8650372765665457; 3.26210755147829; -2.8750565102352179; -0.60529706392899174; 2.9918399880007103; -1.3913747829982035; -6.3286350313135618; 2.1076734065113518; -3.4658154177561142; -4.5171855004796431; 2.4993281269426362; 1.8170869383488675; -4.6101297902501717; -6.5372888197882695; 1.7268999668675911 |
+                        0 : float |] | [| | 0 : float |] : array float |]
+
+Goal True.
+  pose (PArray.concretize (logits (tensor_of_list [0; 1]%uint63))) as v.
+  cbv beta delta [logits PArray.checkpoint] in v.
+  set (k := PArray.concretize _) in (value of v) at 2.
+  Time vm_compute in k.
+  subst k.
+  set (k := PArray.concretize _) in (value of v) at 2.
+  Time vm_compute in k.
+  subst k.
+  repeat match (eval cbv delta [v] in v) with
+         | context V[let x := ?val in @?k x]
+           => lazymatch val with
+              | context[PArray.concretize ?val] => fail 1 val
+              | _ => idtac
+              end;
+              let V := context V[match val with x => k x end] in
+              change V in (value of v); cbv beta in v
+         end.
+  set (k := PArray.concretize _) in (value of v) at 2.
+  Time vm_compute in k.
+  subst k.
+  repeat match (eval cbv delta [v] in v) with
+         | context V[let x := ?val in @?k x]
+           => lazymatch val with
+              | context[PArray.concretize ?val] => fail 1 val
+              | _ => idtac
+              end;
+              let V := context V[match val with x => k x end] in
+              change V in (value of v); cbv beta in v
+         end.
+  set (k := PArray.concretize _) in (value of v) at 2.
+  lazymatch (eval cbv delta [k] in k) with
+  | PArray.concretize (block0 ?x)
+    => set (k0 := x) in (value of k); set (k1 := block0 k0) in (value of k)
+  end.
+  cbv beta delta [block0] in k1.
+  cbv beta zeta in k1.
+  cbv beta delta [transformer_block_attn_only_out] in k1.
+  cbv beta zeta in k1.
+  Timeout 10 Time vm_compute in k.
+  cbv beta delta [PArray.checkpoint] in k3.
+  set (k_tmp := PArray.concretize _) in (value of k3).
+  Time vm_compute in k_tmp.
+  subst k_tmp.
+  lazymatch (eval cbv delta [k1] in k1) with
+  | (_ + ?x)%core
+    => set (k2 := x) in (value of k1)
+  end.
+  clear -k2.
+  cbv beta delta [attn_out] in k2.
+  cbv beta zeta in k2.
+  cbv beta delta [PArray.checkpoint] in k2.
+  set (k_tmp := PArray.concretize _) in (value of k2).
+  (*Set NativeCompute Profiling.
+  Set NativeCompute Timing.*)
+  Time vm_compute in k_tmp.
+  subst k_tmp.
+  lazymatch (eval cbv delta [k2] in k2) with
+  | PArray.checkpoint (map' ?f ?x + ?y)%core
+    => set (k3 := x) in (value of k2);
+       set (k4 := y) in (value of k2)
+  end.
+  cbv [z] in k3.
+  cbv beta delta [PArray.checkpoint] in k3.
+  set (k_tmp := PArray.concretize _) in (value of k3).
+  Time vm_compute in k_tmp.
+  subst k_tmp.
+  HERE
+  cbv beta delta [z] in k3.
+  cbv beta zeta in k3.
+  let k := k3 in
+  lazymatch (eval cbv delta [k] in k) with
+  | PArray.checkpoint (map2' ?f ?x ?y)%core
+    => let k1 := fresh "k" in
+       let k2 := fresh "k" in
+       set (k1 := x) in (value of k);
+       set (k2 := y) in (value of k)
+  end.
+  cbv beta delta [v] in *.
+  cbv beta zeta in k1.
+  cbv beta delta [value_input key_input query_input add_head_dimension] in *.
+  cbv beta zeta iota in k1, k2.
+  cbv beta delta [transformer_block_ln1] in *.
+  cbv beta zeta iota in k1, k2.
+  set (lnv := layernorm _ _ _ _) in *.
+  cbv beta delta [layernorm pattern] in *.
+  cbv beta iota zeta in lnv.
+  cbv beta delta [PArray.checkpoint] in lnv.
+  set (k_tmp := PArray.concretize _) in (value of lnv).
+  Time vm_compute in k_tmp.
+  subst k_tmp.
+  cbv beta delta [PArray.checkpoint] in k3.
+  set (k_tmp := PArray.concretize _) in (value of k3).
+  Time vm_compute in k_tmp.
+  subst k_tmp.
+  cbv beta delta [PArray.checkpoint] in k1.
+  set (k_tmp := PArray.concretize _) in (value of k1).
+  Time vm_compute in k_tmp.
+  subst k_tmp.
+  cbv beta zeta in k2.
+  cbv beta delta [PArray.checkpoint] in k2.
+  set (k_tmp := PArray.concretize _) in (value of k2).
+  Time vm_compute in k_tmp.
+  subst k_tmp.
+
+  set (
+  cbv [einsum_input] in k1.
+  Timeout 5 Compute PArray.concretize k3.
+               (*
+  cbv beta delta [Shape.hd Shape.nil Shape.tl Shape.snoc fst snd Shape.cons Shape.app Nat.radd Tensor.raw_get] in k1.
+
+  cbv beta iota zeta in k1.
+  Set Printing All.
+
+  cbn [fst snd] in k1.
+
+
+  pose
+  Timeout 5 Compute PArray.concretize lnv.
+  pose (lnvc := PArray.concretize lnv).
+  vm_compute in lnvc.
+  vm_compute in lnv.
+  clear -lnv.
+  set (lnlv := layernorm_linpart _) in *.
+  cbv beta delta [layernorm_linpart] in *.
+  set (mv := reduce_axis_m1 _ _) in *.
+  cbv beta delta [reduce_axis_m1] in *.
+  clear -mv.
+  cbv beta iota in mv.
+  set (mv' := reduce_axis_m1' _ _) in *.
+  clear -mv'.
+  cbv beta delta [reduce_axis_m1'] in *.
+  vm_compute Shape.tl in mv'.
+  set (k_tmp := reshape_snoc_split) in *.
+  cbv in k_tmp; subst k_tmp.
+  cbv beta iota in mv'.
+  cbv beta delta [map] in mv'.
+  pose (PArray.concretize mv') as mv'c.
+  vm_compute in mv'c.
+  cbv [PArray.concretize Shape.snoc init_default] in mv'c.
+  set (k_tmp := _ <=? max_length) in *.
+  vm_compute in k_tmp; subst k_tmp; cbv beta iota in mv'c.
+  vm_compute make in mv'c.
+  cbv -[mv'] in mv'c.
+  subst mv'.
+  cbv beta iota zeta in mv'c.
+  cbv [mean] in mv'c.
+  vm_compute inject_Z_coer in mv'c.
+  cbv [raw_get] in mv'c.
+  cbv [RawIndex.snoc RawIndex.nil] in mv'c.
+  cbv [sum] in mv'c.
+  cbv [map_reduce] in mv'c.
+  Timeout 5 cbv -[add Q_has_add k0 Qdiv] in mv'c.
+  Time repeat (time (set (k0v := k0 _) in (value of mv'c) at 1;
+                     timeout 5 vm_compute in k0v; subst k0v)).
+  Time vm_compute in mv'c.
+.
+  set (k0v := k0 _) in (value of mv'c) at 1.
+  timeout 5 vm_compute in k0v; subst k0v.
+  set (k0v := k0 _) in (value of mv'c) at 1.
+  timeout 5 vm_compute in k0v; subst k0v.
+  set (k0v := k0 _) in (value of mv'c) at 1.
+  timeout 5 vm_compute in k0v; subst k0v.
+  set (k0v := k0 _) in (value of mv'c) at 1.
+  timeout 5 vm_compute in k0v; subst k0v.
+  do 10 (set (k0v := k0 _) in (value of mv'c) at 1;
+          timeout 5 vm_compute in k0v; subst k0v).
+  do 10 (set (k0v := k0 _) in (value of mv'c) at 1;
+          timeout 5 vm_compute in k0v; subst k0v).
+  do 10 (set (k0v := k0 _) in (value of mv'c) at 1;
+          timeout 5 vm_compute in k0v; subst k0v).
+  clear -k0v.
+  set (val := (_ + _)%core) in (value of k0) at 1.
+  cbv [ltb] in *.
+  vm_compute RawIndex.repeat in k0.
+  vm_compute Shape.snoc in k0.
+  vm_compute PArray.abstract in k0.
+  clearbody val.
+  vm_compute in val.
+  vm_compute RawIndex in *.
+
+  vm_compute in k0v.
+(*
+  generalize dependent (_ + _)
+  cbv in k0.
+  cbv [RawIndex
+  vm_compute in k0v.
+  cbv in k0v.
+  Timeout 5 vm_compute in k0v.
+  vm_compute in k0v.
+  subst k0.
+  Set Printing All.
+  cbv in mv'c.
+  vm_compute
+
+  cbv -
+  cbv [reshape_snoc_split] in mv'.
+  cbv [reshape_snoc_split] in mv'.
+
+  Timeout 5 Compute PArray.concretize mv'.
+  cbv beta delta [reduce_axis_m1'] in *.
+
+  Timeout 5 Compute PArray.concretize mv.
+  let k := k1 in
+  let k1 := fresh "k" in
+  let k2 := fresh "k" in
+  lazymatch (eval cbv delta [k] in k) with
+  | (map2' ?f ?x ?y)%core
+    => set (k1 := x) in (value of k);
+       set (k2 := y) in (value of k)
+  end.
+
+
+
+  set (k2 := attn_out _ _ _
+  Time native_compute in k.
+  Time vm_compute in k.
+  subst k.
+
+  cbv
+  set (k := PArray.concretize _) in (value of v) at 2.
+  Time vm_compute in k.
+  subst k.
+
+Time Timeout 5 Compute PArray.concretize (logits (tensor_of_list [0; 1]%uint63)).
+Compute PArray.concrete_tensor
+
+Compute PArray.concretize (embed (tensor_of_list [0; 1]%uint63)).
+Compute PArray.concretize (pos_embed (tensor_of_list [[0; 1]]%uint63) : tensor FLOAT [1; cfg.n_ctx; cfg.d_model]).
+*)
+*)*)
