theories/MaxOfTwoNumbersSimpler/TheoremStatement.v
@@ -1,0 +1,34 @@
+From Coq Require Import Floats Sint63 Uint63 QArith List PArray.
+From NeuralNetInterp.Torch Require Import Tensor Einsum Slicing.
+From NeuralNetInterp.Util Require Import Default Pointed PArray List Notations Arith.Classes Arith.Instances Bool.
+(*From NeuralNetInterp.Util Require Import Default Pointed PArray List Notations Arith.Classes Arith.Instances Bool.
+From NeuralNetInterp.Util Require Nat Wf_Uint63.
+From NeuralNetInterp.TransformerLens Require Import HookedTransformer.
+Import Util.Nat.Notations.
+Import Util.Wf_Uint63.LoopNotation.
+Import Util.Wf_Uint63.
+Import Util.Wf_Uint63.Reduction.
+Import Arith.Instances.Truncating.
+Local Open Scope float_scope.
+Local Open Scope list_scope.
+Set Implicit Arguments.
+Import ListNotations.*)
+From NeuralNetInterp.MaxOfTwoNumbersSimpler Require Import Model Parameters Heuristics.
+Local Open Scope raw_tensor_scope.
+
+Definition total : int := Eval vm_compute in Shape.item (Shape.reshape (shape_of all_tokens)).
+Definition expected_correct : int := Eval vm_compute in total - Uint63.of_Z 0 (* (List.length Heuristics.incorrect_results)*).
+Definition totalf : float := Eval vm_compute in PrimFloat.of_uint63 total.
+Definition expected_correctf : float := Eval vm_compute in PrimFloat.of_uint63 expected_correct.
+Definition expected_accuracy : float := Eval vm_compute in expected_correctf / totalf.
+
+Definition real_accuracy : float
+  := Tensor.item (acc_fn (return_per_token := false) (logits all_tokens) all_tokens).
+
+Definition error : float := Eval cbv in (20 / totalf)%float.
+
+Module Accuracy.
+  Local Notation abs := (@abs float float_has_abs) (only parsing).
+  Notation best := ((abs (real_accuracy - expected_accuracy) =? 0)%float = true)
+                     (only parsing).
+End Accuracy.
