theories/MaxOfTwoNumbersSimpler/Theorems/Attempt_01_BruteForce.v
@@ -1,0 +1,28 @@
+From Coq Require Import Floats Sint63 Uint63 QArith Lia List PArray Derive.
+From NeuralNetInterp.Torch Require Import Tensor Einsum Slicing.
+From NeuralNetInterp.Util Require Import Pointed.
+From NeuralNetInterp.Util.Arith Require Import Classes Instances FloatArith.Definitions.
+From NeuralNetInterp.Torch Require Import Tensor.Instances.
+From NeuralNetInterp.MaxOfTwoNumbersSimpler Require Import Parameters Model Heuristics TheoremStatement Model.Instances.
+From NeuralNetInterp.MaxOfTwoNumbersSimpler.Computed Require Import AllLogits.
+Local Open Scope uint63_scope.
+Local Open Scope core_scope.
+
+Derive computed_accuracy SuchThat (computed_accuracy = real_accuracy) As computed_accuracy_eq.
+Proof.
+  cbv [real_accuracy].
+  etransitivity; revgoals.
+  { apply Tensor.item_Proper; intro.
+    eapply Model.acc_fn_Proper; repeat intro; subst; [ | reflexivity .. ].
+    apply all_tokens_logits_eq. }
+  Time vm_compute; reflexivity.
+Defined.
+
+Compute abs (computed_accuracy - expected_accuracy). (*      = 0.0023193359375%float *)
+Compute (abs (computed_accuracy - expected_accuracy) * totalf)%float. (* = 19 *) (* probably from floating point assoc issues, etc *)
+Compute Qred (PrimFloat.to_Q (computed_accuracy * totalf)) / Qred (PrimFloat.to_Q totalf). (*      = 8154 # 8192 *)
+Theorem good_accuracy : TheoremStatement.Accuracy.best (* (abs (real_accuracy - expected_accuracy) <? error)%float = true *).
+Proof.
+  rewrite <- computed_accuracy_eq.
+  vm_compute; reflexivity.
+Qed.
